\documentclass{article}
\usepackage[utf8]{inputenc}

\usepackage[a4paper, total={6in, 8in}]{geometry}

\author{Lara Lusa, Crt Ahlin}
\date{October 2016}

\title{Proposals for a cyclic cubic spline}
\usepackage{amsmath}

\begin{document}

\maketitle

\section{Definition of cubic splines}
\begin{gather}
s(x)=\gamma_0+\gamma_1 X + \gamma_2 X^2 + \gamma_3 X^3 + \beta_1 (X-t_1)^3_{+}+ \beta_2 (X-t_2)^3_{+}+ ... +\beta_k (X-t_k)^3_{+}+ \\
s(x)=\gamma_0+\gamma_1 X + \gamma_2 X^2 + \gamma_3 X^3 + \sum_{j=1}^k\beta_j (X-t_j)^3_{+}
\end{gather}

%Linearity for $x\le t_1$ implies that $\gamma_2=\gamma_3=0$

%Linearity for $x \ge t_k$ implies that the spline can be defined using k-2 coefficients, re-parametrizing the function

For \(x \le t_1\) 

\begin{gather*} 
s(x)=\gamma_0+\gamma_1 X + \gamma_2 X^2 + \gamma_3 X^3 \\
s^{\prime}(x)=\gamma_1 + 2\gamma_2 X + 3\gamma_3 X^2  \\
s^{\prime\prime}(x)= 2\gamma_2  + 6\gamma_3 X  
\end{gather*}

For $x \ge t_k$ 
\begin{gather*}
s(x)=\gamma_0+\gamma_1 X + \gamma_2 X^2 + \gamma_3 X^3 + \sum_{j=1}^k\beta_j (X-t_j)^3 \\
s^{\prime}(x)=\gamma_1 + 2\gamma_2 X + 3\gamma_3 X^2 + 3\sum_{j=1}^k\beta_j (X-t_j)^2 \\
s^{\prime\prime}(x)= 2\gamma_2  + 6\gamma_3 X + 6\sum_{j=1}^k\beta_j (X-t_j) \\
\end{gather*}


\section{Constraining Cubic splines to achieve the same estimated value at the beginning and end of the cycle}

Imposing the constraints

\[ s(x_{min})=s(x_{max}) \]

\begin{gather*}
\gamma_0+\gamma_1 X_{min} + \gamma_2 X_{min}^2 + \gamma_3 X_{min}^3 = 
\gamma_0+\gamma_1 X_{max} + \gamma_2 X_{max}^2 + \gamma_3 X_{max}^3 + \sum_{j=1}^k\beta_j (X_{max}-t_j)^3 \\
\gamma_1 (X_{min}-X_{max}) = 
\gamma_2 (X_{max}^2-X_{min}^2) + \gamma_3 (X_{max}^3-X_{min}^3) + \sum_{j=1}^k\beta_j (X_{max}-t_j)^3 \\
\gamma_1  = - \gamma_2 \frac{(X_{max}^2-X_{min}^2)}{(X_{max}-X_{min})} - \gamma_3 \frac{(X_{max}^3-X_{min}^3)}{(X_{max}-X_{min})} - \frac{\sum_{j=1}^k\beta_j (X_{max}-t_j)^3}{(X_{max}-X_{min})} \\
\gamma_1  = - \gamma_2 (X_{max}+X_{min})- \gamma_3 (X_{max}^2+X_{max}X_{min}+X_{min}^2) - \frac{\sum_{j=1}^k\beta_j (X_{max}-t_j)^3}{(X_{max}-X_{min})} \\
\gamma_1  = -\frac{1}{X_{max}-X_{min}} \left(\gamma_2 (X^2_{max}-X^2_{min})+ \gamma_3 (X_{max}^3-X^3_{min}) + \sum_{j=1}^k\beta_j (X_{max}-t_j)^3\right)
\end{gather*}
    
Additionally constraining 

\[s^{\prime}(x_{min})=s^{\prime}(x_{max})\]

\begin{gather*}
\gamma_1 + 2\gamma_2 X_{min} + 3\gamma_3 X_{min}^2 = 
\gamma_1 + 2\gamma_2 X_{max} + 3\gamma_3 X_{max}^2 + 3\sum_{j=1}^k\beta_j (X_{max}-t_j)^2 \\
\gamma_2 (X_{min}-X_{max}) = 
  3/2\gamma_3 (X_{max}^2-X_{min}^2) + 3/2\sum_{j=1}^k\beta_j (X_{max}-t_j)^2 \\
\gamma_2  = 
  - 3/2 \gamma_3 \frac{(X_{max}^2-X_{min}^2)}{(X_{max}-X_{min})} - 3/2\frac{\sum_{j=1}^k\beta_j (X_{max}-t_j)^2}{(X_{max}-X_{min})} \\
\gamma_2=-\frac{3}{2 (X_{max}-X_{min})} \left( \gamma_3 (X^2_{max}-X^2_{min}) + \sum_{j=1}^k\beta_j (X_{max}-t_j)^2 )    \right) \\
\gamma_2  = 
  - 3/2 \gamma_3 (X_{max}+X_{min}) - 3/2\frac{\sum_{j=1}^k\beta_j (X_{max}-t_j)^2}{(X_{max}-X_{min})} 
\end{gather*}

Finaly, we have to constrain

\[ s^{\prime\prime}(x_{min})=s^{\prime\prime}(x_{max}) \]

\begin{gather*}
2\gamma_2  + 6\gamma_3 X_{min}=
2\gamma_2  + 6\gamma_3 X_{max} + 6\sum_{j=1}^k\beta_j (X_{max}-t_j) \\
\gamma_3 (X_{min}-X_{max})=\sum_{j=1}^k\beta_j (X_{max}-t_j)
\end{gather*}

Deriving \( \gamma_3 \)

\[
\gamma_3 =\frac{\sum_{j=1}^k\beta_j (X_{max}-t_j)}{X_{min}-X_{max}}=-\frac{\sum_{j=1}^k\beta_j (X_{max}-t_j)}{X_{max}-X_{min}}
\]


\clearpage
Summarizing the results

\begin{gather}
\gamma_3 =-\frac{\sum_{j=1}^k\beta_j (X_{max}-t_j)}{X_{max}-X_{min}} \\
\gamma_2=-\frac{3}{2 (X_{max}-X_{min})} \left( \gamma_3 (X^2_{max}-X^2_{min}) + \sum_{j=1}^k\beta_j (X_{max}-t_j)^2     \right) \\
\gamma_1  = -\frac{1}{X_{max}-X_{min}} \left(\gamma_2 (X^2_{max}-X^2_{min})+ \gamma_3 (X_{max}^3-X^3_{min}) + \sum_{j=1}^k\beta_j (X_{max}-t_j)^3\right)
\end{gather}

We already have \( \gamma_3 \) expressed as a fnuction of \( \beta_j \). 

Deriving \( \gamma_2 \) as a function of \( \beta_j \)

\begin{gather*}
\gamma_2=-\frac{3}{2 (X_{max}-X_{min})} \left( \gamma_3 (X^2_{max}-X^2_{min}) + \sum_{j=1}^k\beta_j (X_{max}-t_j)^2     \right) \\
\gamma_3 =-\frac{\sum_{j=1}^k\beta_j (X_{max}-t_j)}{X_{max}-X_{min}} \\
\gamma_2=-\frac{3}{2 (X_{max}-X_{min})} \left( \left( -\frac{\sum_{j=1}^k\beta_j (X_{max}-t_j)}{X_{max}-X_{min}} \right)  (X^2_{max}-X^2_{min}) + \sum_{j=1}^k\beta_j (X_{max}-t_j)^2     \right) \\
\gamma_2= \frac{3(X^2_{max}-X^2_{min}) \sum_{j=1}^k\beta_j (X_{max}-t_j) }{2 (X_{max}-X_{min})^2} 
-\frac{3  \sum_{j=1}^k\beta_j (X_{max}-t_j)^2  }{2 (X_{max}-X_{min})} \\
\gamma_2= \frac{3(X_{max}+X_{min}) \sum_{j=1}^k\beta_j (X_{max}-t_j) }{2 (X_{max}-X_{min})} 
-\frac{3  \sum_{j=1}^k\beta_j (X_{max}-t_j)^2  }{2 (X_{max}-X_{min})}    
\end{gather*}

\clearpage 
Deriving \(\gamma_1 \) as a function of \( \beta_j \)

\[
\gamma_1  = -\frac{1}{X_{max}-X_{min}} \left(\gamma_2 (X^2_{max}-X^2_{min})+ \gamma_3 (X_{max}^3-X^3_{min}) + \sum_{j=1}^k\beta_j (X_{max}-t_j)^3\right)
\]

\begin{equation*}
\begin{aligned}
 \gamma_1  = &    -\frac{1}{X_{max}-X_{min}} \Biggl( \\
&  (X^2_{max}-X^2_{min}) \left(\frac{3(X_{max}+X_{min}) \sum_{j=1}^k\beta_j (X_{max}-t_j) }{2 (X_{max}-X_{min})} 
-\frac{3  \sum_{j=1}^k\beta_j (X_{max}-t_j)^2  }{2 (X_{max}-X_{min})} \right) + \\
%&& \gamma_3 (X_{max}^3-X^3_{min})\\
& -\frac{\sum_{j=1}^k\beta_j (X_{max}-t_j)}{X_{max}-X_{min}} (X_{max}^3-X^3_{min})\\
& + \sum_{j=1}^k\beta_j (X_{max}-t_j)^3\Biggr)\\
\end{aligned}
\end{equation*}


\begin{multline*}
\gamma_1  = -\frac{1}{X_{max}-X_{min}} \Biggl( \\ 
(X^2_{max}-X^2_{min}) \left(\frac{3(X_{max}+X_{min}) \sum_{j=1}^k\beta_j (X_{max}-t_j) }{2 (X_{max}-X_{min})} 
-\frac{3  \sum_{j=1}^k\beta_j (X_{max}-t_j)^2  }{2 (X_{max}-X_{min})} \right) + \\
-\frac{\sum_{j=1}^k\beta_j (X_{max}-t_j)}{X_{max}-X_{min}} (X_{max}^3-X^3_{min}) + \\ \sum_{j=1}^k\beta_j (X_{max}-t_j)^3 \Biggr)
\end{multline*}

% TODO: which variant to use - aligned or multiline?
%
%\begin{equation*}
%\begin{aligned}
% \gamma_1  = &    -\frac{1}{X_{max}-X_{min}} \Biggl( \\
%&  (X_{max}+X_{min}) \left(\frac{3(X_{max}+X_{min}) \sum_{j=1}^k\beta_j (X_{max}-t_j) }{2} 
%-\frac{3  \sum_{j=1}^k\beta_j (X_{max}-t_j)^2  }{2} \right) + \\
%& -\frac{\sum_{j=1}^k\beta_j (X_{max}-t_j)}{X_{max}-X_{min}} (X_{max}^3-X^3_{min})\\
%& + \sum_{j=1}^k\beta_j (X_{max}-t_j)^3\Biggr)\\
%\end{aligned}
%\end{equation*}


\begin{equation*}
\begin{aligned}
 \gamma_1  = &    -\frac{1}{X_{max}-X_{min}} \Biggl( \\
&   \frac{3(X_{max}+X_{min})^2 \sum_{j=1}^k\beta_j (X_{max}-t_j) }{2} 
-\frac{3(X_{max}+X_{min})  \sum_{j=1}^k\beta_j (X_{max}-t_j)^2  }{2}  + \\
& -\frac{\sum_{j=1}^k\beta_j (X_{max}-t_j)}{X_{max}-X_{min}} (X_{max}^3-X^3_{min})\\
& + \sum_{j=1}^k\beta_j (X_{max}-t_j)^3\Biggr)\\
\end{aligned}
\end{equation*}

\begin{equation*}
\begin{aligned}
s(x)=& \gamma_0+\gamma_1 X + \gamma_2 X^2 + \gamma_3 X^3 + \sum_{j=1}^k\beta_j (x-t_j)_{+}^3 \\
& =\gamma_0+ \\
&  -\frac{X}{X_{max}-X_{min}} \Biggl(  \\
&   \frac{3(X_{max}+X_{min})^2 \sum_{j=1}^k\beta_j (X_{max}-t_j) }{2} +\\
& - \frac{3(X_{max}+X_{min})  \sum_{j=1}^k\beta_j (X_{max}-t_j)^2  }{2} + \\
& -\frac{\sum_{j=1}^k\beta_j (X_{max}-t_j)}{X_{max}-X_{min}} (X_{max}^3-X^3_{min}) \\
& + \sum_{j=1}^k\beta_j (X_{max}-t_j)^3 \Biggr)\\
& +  \left( \frac{3(X_{max}+X_{min}) \sum_{j=1}^k\beta_j (X_{max}-t_j) }{2 (X_{max}-X_{min})} 
 -\frac{3  \sum_{j=1}^k\beta_j (X_{max}-t_j)^2  }{2 (X_{max}-X_{min})}\right) X^2\\
&  - \left( \frac{\sum_{j=1}^k\beta_j (X_{max}-t_j)}{X_{max}-X_{min}} \right) X^3\\
& + \sum_{j=1}^k\beta_j (x-t_j)_{+}^3\\
\end{aligned}
\end{equation*}

\[ s(x)=\gamma_0+\sum_{j=1}^k\beta_j s_j(x) \]
 
\[ s_j(x)=a_jx+b_j x^2+c_j x^3+ (x-t_j)_{+}^3 \]

with 

% TODO: which of the three variants of style below to use?
\begin{equation*}
\begin{aligned}
a_j=
&  -\frac{1}{X_{max}-X_{min}} \Biggl(  \\
&   \frac{3(X_{max}+X_{min})^2  (X_{max}-t_j) }{2} +\\
& - \frac{3(X_{max}+X_{min})   (X_{max}-t_j)^2  }{2} + \\
& -\frac{(X_{max}-t_j)}{X_{max}-X_{min}} (X_{max}^3-X^3_{min}) \\
& + (X_{max}-t_j)^3 \Biggr)=\\
&  -\frac{1}{X_{max}-X_{min}} \Biggl(  \\
&   \frac{X^2_{max}+X^2_{min}+4X_{max}X_{min}  }{2} (X_{max}-t_j)+\\
& - \frac{3(X_{max}+X_{min})}{2}(X_{max}-t_j)^2 + \\
& + (X_{max}-t_j)^3 \Biggr)
\end{aligned}
\end{equation*}

% variatn multiline
%\begin{multline}
%a_j = 
%  -\frac{1}{X_{max}-X_{min}} \Biggl(  
%   \frac{3(X_{max}+X_{min})^2  (X_{max}-t_j) }{2} +
% - \frac{3(X_{max}+X_{min})   (X_{max}-t_j)^2  }{2} + \\
% -\frac{(X_{max}-t_j)}{X_{max}-X_{min}} (X_{max}^3-X^3_{min}) 
% + (X_{max}-t_j)^3 \Biggr)=\\
%  -\frac{1}{X_{max}-X_{min}} \Biggl(  \\
%   \frac{X^2_{max}+X^2_{min}+4X_{max}X_{min}  }{2} (X_{max}-t_j)+\\
% - \frac{3(X_{max}+X_{min})}{2}(X_{max}-t_j)^2 + \\
% + (X_{max}-t_j)^3 \Biggr)
%\end{multline}

% variant split
%\begin{equation*}
%\begin{split}
%a_j & = -\frac{1}{X_{max}-X_{min}} \Biggl( \\
%& \frac{3(X_{max}+X_{min})^2  (X_{max}-t_j) }{2} + \\
%& -\frac{3(X_{max}+X_{min})   (X_{max}-t_j)^2  }{2} + \\
%& -\frac{(X_{max}-t_j)}{X_{max}-X_{min}} (X_{max}^3-X^3_{min})+ \\
%& + (X_{max}-t_j)^3 \Biggr) \\
%& =  -\frac{1}{X_{max}-X_{min}} \Biggl(  \\
%& \frac{X^2_{max}+X^2_{min}+4X_{max}X_{min}  }{2} (X_{max}-t_j)+ \\
%& -\frac{3(X_{max}+X_{min})}{2}(X_{max}-t_j)^2 + \\
%& +(X_{max}-t_j)^3 \Biggr)
%\end{split}
%\end{equation*}

%\begin{equation} \label{eq1}
%\begin{split}
%a_j & = \\ &-\frac{1}{X_{max}-X_{min}} \Biggl( \\
%    & 3 +3 +3 \Biggr)
%\end{split}
%\end{equation}

\[ b_j= \frac{3(X_{max}+X_{min}) (X_{max}-t_j) }{2 (X_{max}-X_{min})} 
 -\frac{3   (X_{max}-t_j)^2  }{2 (X_{max}-X_{min})} \]

\[ c_j= - \frac{(X_{max}-t_j)}{X_{max}-X_{min}} \]


Assuming that the period of x is defined on \( [0, T] \) (i.e., \( X_{min}=0, X_{max}=T \) ) 
\(a_j \), \(b_j\) and \(c_j\) simplify to 

\begin{align*}
a_j & = -\frac{1}{T} \bigl(  \frac{3T^2  (T-t_j) }{2} - \frac{3T (T-t_j)^2  }{2} -\frac{T^3(T-t_j)}{T}  + (T-t_j)^3 \bigr) = \\
 & = - \frac{3T(T-t_j) }{2} + \frac{3(T-t_j)^2  }{2} +\frac{T(T-t_j)}{1}  - \frac{(T-t_j)^3}{T} 
- \frac{T(T-t_j) }{2} + \frac{3(T-t_j)^2  }{2}  
 - \frac{(T-t_j)^3}{T} \\ 
b_j & = \frac{3(T-t_j) }{2} 
 -\frac{3   (T-t_j)^2  }{2T} \\
c_j & = -  \frac{T-t_j}{T}, \\
\end{align*}

which are the same values reported by Zhang et al., 2000 (but note that $c_j$ was reported omitting the minus sign in the original paper, which should be regarded as a typo, as the equations produce a periodic cubic spline using the formulas reported above.)

\end{document}



